examples/cellio/CellioAll.v
@@ -1,0 +1,113 @@
+Require Import CRIS Cancel.
+Require Import ImpPrelude.
+Require Import CellioHeader MainHeader InputHeader FooHeader.
+Require Import CellioA CellioI MainA MainI InputA.
+Require Import InputASpec FooASpec.
+Require Import CellioIAproof MainIAproof.
+
+Module CellioAll. Section CellioAll.
+  Import inv_instances.
+  Local Instance Γ : HRA := ##[invΓ; CellioAΓ].
+  Local Instance Σ : GRA := ##[invΣ; Γ].
+  
+  (* Definition stb_add stb0 stb1: Sk.t -> string -> option fspec :=
+    fun sk fn =>
+      match stb0 sk fn, stb1 sk fn with
+      | Some fsp, None => Some fsp
+      | None, Some fsp => Some fsp
+      | _, _ => None
+      end. *)
+
+  Local Definition smod_src : SMod.t := MainA.Mod ☆ CellioA.Mod ☆ InputA.Mod.
+  Local Definition ginv : Sk.t → invspec := λ _ _, True%I.
+  Local Definition stb : Sk.t → string → option fspec := stb_global smod_src.
+  Local Definition mod_cancel : HMod.t := SModCancel.to_hmod smod_src.
+  Local Definition mod_src : HMod.t := SMod.to_hmod ginv stb smod_src.
+  Local Definition mod_tgt : HMod.t := MainI.t ★ CellioI.t ★ (InputA.t ginv stb).
+
+  Local Definition main_fsp : fspec := fspec_trivial.
+  Local Definition init_cond : Sk.t → iProp Σ := MainA.InitCond ∗∗ CellioA.InitCond ∗∗ InputA.InitCond.
+  Local Definition skeleton : Sk.t := Sk.add CellioSK.t MainSK.t.
+
+  (* Apply cancellation to linked spec module *)
+  Lemma cancel_src :
+    refines (mod_cancel, init_cond ∗∗ (λ _, main_fsp.(precond) 0 tt tt↑ tt↑)) 
+            ((mod_src, init_cond) : HMod.modc).
+  Proof.
+    eapply cancellation; try by econs.
+    i. iIntros "%POST". iPureIntro.
+    des; eauto.
+  Qed.
+
+  (* Refinement between spec/impl of whole program (linked module) *)
+  Lemma src_tgt : refines (mod_src, init_cond) (mod_tgt, const(emp)%I).
+  Proof.
+    (* consider identical modules in src/tgt as context (InputA) *)
+    eapply ctxr_refines.
+    rewrite -[(_, const (emp%I))]hmod_addc_empty_r /init_cond -hmod_addc_assoc.
+    rewrite /mod_src /mod_tgt !add_interp_comm -!hmod_add_assoc /InputA.t.
+    unseal CRIS. eapply ctxr_frameR, ctxr_cond_frameR.
+    (* solve by transitivity:
+      MainI ★ CellioI ⊆ MainI ★ CellioA ⊆ MainA ★ CellioA 
+    *)
+    etrans.
+    {
+      (* MainI ★ CellioA ⊆ MainA ★ CellioA *)
+      rewrite -[(SMod.to_hmod _ _ MainA.Mod)](Seal.sealing_eq CRIS) -[(SMod.to_hmod _ _ CellioA.Mod)](Seal.sealing_eq CRIS).
+      instantiate (1:= (MainI.t ★ (CellioA.t ginv stb), (const(emp%I)) ∗∗ CellioA.InitCond)).
+      eapply ctxr_cond_frameR, main_adequacy, MainIA.sim.
+      {
+        admit. 
+      }
+      {
+        i. rewrite /InputAS.Stb. unseal CRIS. econs; first prove_nodup.
+        ii; rewrite -FIND /stb /stb_global /smod_src //=. des_ifs; ss; des_ifs.
+      }
+    }
+    (* MainI ★ CellioI ⊆ MainI ★ CellioA 
+      by CellioI ⊆ctx CellioA *)
+    rewrite -[(_, const (emp%I))]hmod_addc_empty_r.
+    eapply ctxr_frameL, ctxr_cond_frameL, main_adequacy, CellioIA.sim. 
+    i. rewrite /InputAS.Stb. unseal CRIS. econs; first prove_nodup.
+    ii; rewrite -FIND /stb /stb_global /smod_src //=.
+    des_ifs; ss; des_ifs.
+  (* Qed. *)
+  Admitted.
+
+  Lemma cancel_tgt :
+    refines (mod_cancel, init_cond ∗∗ (λ _, main_fsp.(precond) 0 tt tt↑ tt↑))
+            (mod_tgt, const(emp)%I).
+  Proof.
+    etrans.
+    { eapply cancel_src. }
+    { eapply src_tgt. }
+  Qed.
+
+  Local Definition initial_resource : Σ := MainAS.init_res ⋅ CellioAS.init_res.
+  Lemma initial_resource_valid : ✓ initial_resource.
+  Proof.
+    rewrite /initial_resource /MainAS.init_res /CellioAS.init_res -own.iRes_singleton_op.
+    apply discrete_fun_singleton_valid, allocs.allocs_frag_valid,
+      cmra_transport_valid, excl_auth_valid.
+  Qed.
+
+  Theorem behavioral_refinement :
+    ∃ target_resource, refines_modsem
+      (HModSem.to_mod ((HMod.modsem mod_cancel) skeleton) initial_resource)
+      (HModSem.to_mod ((HMod.modsem mod_tgt) skeleton) target_resource).
+  Proof.
+    move: (cancel_tgt)=>H; rewrite /refines in H; des; ss.
+    destruct (REF skeleton initial_resource).
+    { rewrite /CellioI.t /MainI.t /skeleton; unseal CRIS; ss. }
+    { rewrite /skeleton /CellioSK.t /MainSK.t; ss; econs; ii; ss; des; ss; prove_nodup. }
+    { apply initial_resource_valid. }
+    { iIntros "I"; rewrite /init_cond /CellioA.init_cond /MainA.init_cond /HMod.addc.
+      rewrite /precond /= /CellioAS.Ready /CellioAS.Ball
+        own.Own_eq own.own_eq /own.Own_def /own.own_def.
+      iDestruct "I" as "[I1 I2]"; iFrame. iSplit; iPureIntro; ss.
+    }
+    { econs; ss; try prove_nodup. }
+    { exists x; des; eauto. }
+  Qed.
+End CellioAll. End CellioAll.
+Print Assumptions CellioAll.behavioral_refinement.
