examples/cellio/InputA.v
@@ -1,0 +1,39 @@
+Require Import CRIS.
+Require Import InputHeader.
+
+Set Implicit Arguments.
+
+Module InputA. Section InputA.
+  Context `{Σ: GRA}.
+
+  Definition input: Any.t -> itree hmodE Any.t :=
+    λ _,
+      i <- trigger (@IO _ Z "Input" tt);;
+      trigger (@IO _ unit "Print" i);;;
+      Ret i↑.
+
+  Definition scopes := [InputName.mn].
+  
+  Definition fnsems : alist string (list string * fspecbody) :=
+    [(InputName.input, (scopes, mk_specbody fspec_trivial input))].
+
+  Program Definition Sem : SModSem.t := {|
+    SModSem.scopes := scopes;
+    SModSem.fnsems := fnsems;
+    SModSem.initial_st := [];
+  |}.
+  Solve All Obligations with prove_scope.
+  Next Obligation. prove_nodup. Qed.
+
+  Definition Mod : SMod.t := {|
+    SMod.modsem := λ _, Sem;
+    SMod.sk := InputSK.t;
+  |}.
+
+  Definition InitCond : Sk.t -> iProp Σ :=
+    λ _, emp%I.
+
+  Variable ginv: Sk.t -> invspec.
+  Variable GlobalStb: Sk.t -> string -> option fspec.
+  Definition t := Seal.sealing CRIS (SMod.to_hmod ginv GlobalStb Mod).
+End InputA. End InputA.
