examples/cellio/InputASpec.v
@@ -1,0 +1,19 @@
+Require Import CRIS.
+
+Require Import InputHeader.
+
+Set Implicit Arguments.
+
+Module InputAS.
+Section InputAS.
+  Context `{Σ: GRA}.
+
+  Definition Stb: alist string fspec :=
+    Seal.sealing CRIS [(InputName.input, fspec_trivial)].
+  
+  Lemma Stb_nodup: List.NoDup (List.map fst Stb).
+  Proof.
+    unfold Stb. unseal CRIS. prove_nodup.
+  Qed.
+
+End InputAS. End InputAS.
